HoareLogic/Sound_Resource_TraceSemantics.v
@@ -1,4 +1,5 @@
 Require Import Coq.Logic.FunctionalExtensionality.
+Require Import Coq.Logic.Classical_Prop.
 Require Import Logic.lib.Coqlib.
 Require Import Logic.GeneralLogic.Base.
 Require Import Logic.MinimunLogic.Syntax.
@@ -23,6 +24,27 @@ Import SeparationLogicNotation.
 Import KripkeModelSingleNotation.
 Import KripkeModelNotation_Intuitionistic.
 
+Lemma thread_local_state_enable_acq_inv {state: Type} {Ac: Action} {Res: Resource} {J: Join state} {state_R: Relation state} {Acr: Action_resource Ac Res} {nAcr: NormalAction_resource Ac Res} {ac_sem: ActionInterpret (state * resources) Ac}:
+  forall Inv r s1 A1 A2 ms,
+    (forall r0 : resource, A1 r0 \/ r = r0 <-> A2 r0) ->
+    ~ A1 r ->
+    thread_local_state_enable Inv (Aacquire_res r) (s1, A1) ms ->
+    exists s2 I f, Inv (r, I) /\ I f /\ join s1 f s2 /\ ms = Terminating (s2, A2).
+Proof.
+  intros.
+  inversion H1; subst.
+  + apply Aacquire_res_inv in H2; subst.
+    exists n, I, f.
+    split; [| split; [| split]]; auto.
+    f_equal.
+    f_equal.
+    extensionality r0; apply prop_ext.
+    specialize (H5 r0); specialize (H r0); tauto.
+  + symmetry in H2; apply Aacquire_Arelease_res in H2; inversion H2.
+  + symmetry in H2; apply Aacquire_Arelease_res in H2; inversion H2.
+  + exfalso; apply H2; exists r; auto.
+Qed.
+
 Section soundness.
 
 Existing Instance unit_kMD.
@@ -30,11 +52,13 @@ Existing Instance unit_kMD.
 Context {P: ProgrammingLanguage}
         {MD: Model}
         {J: Join model}
+        {SA: SeparationAlgebra model}
         {R: Relation model}
         {po_R: PreOrder Krelation}
         {Res: Resource}
         {Ac: Action}
         {Acr: Action_resource Ac Res}
+        {nAcr: NormalAction_resource Ac Res}
         {TS: TraceSemantics P (model * resources) Ac}
         {SAAIr: SAActionInterpret_resource model Ac Res ac_sem}.
 
@@ -71,8 +95,8 @@ Proof.
   destruct H1 as [s1 [s2 [? [? ?]]]].
   specialize (fun ms_post HH => H s1 ms_post H8 (traces_access_intro tr1 _ _ _ H2 HH)).
   specialize (fun ms_post HH => H0 s2 ms_post H9 (traces_access_intro tr2 _ _ _ H5 HH)).
-  clear Tr1 Tr2 H2 H5.
-  induction H6.
+  clear P1 P2 H8 H9 Tr1 Tr2 H2 H5.
+  revert s1 s2 s_pre A H H0 H1 H3 H4 H7; induction H6; intros.
   + inversion H4; subst; clear H4.
     destruct ms_post; subst; inversion H2.
     subst m A.
@@ -85,15 +109,49 @@ Proof.
     exists s1, s2.
     split; [| split]; auto.
   + exfalso.
-    destruct (res_actions_no_race _ _ H2).
+    destruct (res_actions_no_race _ _ H).
     apply (state_enable_race_actions_spec a1 a2 A1 A2 s1 s2 s_pre); auto.
     - intro.
-      rewrite (thread_local_state_enable_non_resource_action Inv) in H10 by auto.
-      specialize (H Error (@trace_access_Error _ _ (ThreadLocal_ActionInterpret_resource _ Inv) _ _ _ H10)).
-      inversion H.
-    - intro.
-      rewrite (thread_local_state_enable_non_resource_action Inv) in H10 by auto.
-      specialize (H0 Error (@trace_access_Error _ _ (ThreadLocal_ActionInterpret_resource _ Inv) _ _ _ H10)).
+      rewrite (thread_local_state_enable_non_resource_action Inv) in H8 by auto.
+      specialize (H0 Error (@trace_access_Error _ _ (ThreadLocal_ActionInterpret_resource _ Inv) _ _ _ H8)).
       inversion H0.
-  + Abort.
-      
+    - intro.
+      rewrite (thread_local_state_enable_non_resource_action Inv) in H8 by auto.
+      specialize (H1 Error (@trace_access_Error _ _ (ThreadLocal_ActionInterpret_resource _ Inv) _ _ _ H8)).
+      inversion H1.
+  + destruct (classic (is_resource_action a1)) as [[?r [? | ?]] | ?].
+    - subst a1.
+      destruct (res_enable_acq_inv _ _ _ _ H) as [? [? ?]].
+      set (A' := fun r0 => A r0 \/ r = r0).
+      apply (@trace_access_Terminating_inv _ _ (ThreadLocal_ActionInterpret_resource _ Inv) (fun sa => exists s' I f, Inv (r, I) /\ I f /\ join s_pre f s' /\ sa = (s', A'))) in H4.
+      Focus 2. {
+        intros.
+        simpl in H10.
+        eapply thread_local_state_enable_acq_inv in H10.
+        2: intro; apply iff_refl.
+        2: specialize (H3 r); tauto.
+        destruct H10 as [s' [I [f ?]]].
+        exists (s', A').
+        split; [| tauto].
+        exists s', I, f; tauto.
+      } Unfocus.
+      destruct H4 as [ms [[s' [I [f [? [? [? HEQ]]]]]] ?]]; subst ms.
+      pose proof join_assoc _ _ _ _ _ (join_comm _ _ _ H2) H11 as [s1' [? ?]].
+      apply (IHtrace_interleave s1' s2 s' A').
+      * intros.
+        apply H0.
+        eapply trace_access_Terminating; [clear HH | exact HH].
+        simpl.
+        eapply thread_local_state_enable_acq; eassumption.
+      * apply H1.
+      * apply join_comm; auto.
+      * intros.
+        specialize (H3 r0); specialize (H5 r0). subst A'. tauto.
+      * exact H12.
+      * intros.
+        specialize (H7 r0); specialize (H5 r0).
+        assert (r = r0 -> ~ A2 r0) by (intros; subst; auto).
+        tauto.
+    - Abort.
+
+End soundness.
